floyd/forward.v
@@ -887,14 +887,14 @@ match goal with
   let n := fresh "n" in evar (n: nat); 
   let sh := fresh "sh" in evar (sh: share);
   assert (PROPx P (LOCALx (tc_environ Delta :: Q) (SEPx (number_list O R))) 
-     |-- (`(numbd n (field_mapsto_ sh (typeof e) fld)) (eval_lvalue e)) * TT) as _;
+     |-- (`(numbd n (field_at_ sh (typeof e) fld)) (eval_lvalue e)) * TT) as _;
   [unfold number_list, n, sh; 
    repeat rewrite numbd_lift1; repeat rewrite numbd_lift2;
    solve [entailer; cancel]
  |  ];
 (**** 12.8 seconds to here ****)
  apply (semax_pre_later (PROPx P (LOCALx Q 
-                (SEPx (replace_nth n R (`(field_mapsto_ sh (typeof e) fld) (eval_lvalue e)))))));
+                (SEPx (replace_nth n R (`(field_at_ sh (typeof e) fld) (eval_lvalue e)))))));
  [ eapply (fast_entail n); [reflexivity | entailer; cancel] | ];
 (**** 14.2 seconds to here  *)
  eapply (semax_store_field_nth _ _ n sh); 
@@ -1216,7 +1216,7 @@ match goal with |- semax ?Delta (|> (PROPx ?P (LOCALx ?Q (SEPx ?R)))) (Sassign (
   let sh := fresh "sh" in evar (sh: share);
   let H := fresh in 
   assert (H: PROPx P (LOCALx (tc_environ Delta :: Q) (SEPx (number_list O R))) 
-     |-- (`(numbd n (field_mapsto_ sh (typeof e) fld)) (eval_lvalue e)) * TT);
+     |-- (`(numbd n (field_at_ sh (typeof e) fld)) (eval_lvalue e)) * TT);
   [unfold number_list;
    repeat rewrite numbd_lift1; repeat rewrite numbd_lift2;
    gather_entail
