progs/verif_sha_init.v
@@ -18,7 +18,7 @@ Lemma body_SHA256_Init: semax_body Vprog Gtot f_SHA256_Init SHA256_Init_spec.
 Proof.
 start_function.
 name c_ _c.
-simpl_typed_mapsto.
+simpl_data_at.
 normalize.
 replace (array_at_ tuint Tsh) with (array_at tuint Tsh (ZnthV tuint nil))
  by (rewrite ZnthV_nil_None; reflexivity).
@@ -33,7 +33,7 @@ forward. (* return; *)
 unfold sha256state_.
 apply exp_right with (map Vint init_registers, 
       (Vint Int.zero, (Vint Int.zero, (nil, Vint Int.zero)))).
-simpl_typed_mapsto.
+simpl_data_at.
 unfold s256_h, s256_Nh,s256_Nl, s256_num, s256_data, fst,snd.
 entailer!.
 exists Int.zero, Int.zero; repeat split; reflexivity.
